Add a MReprGhost effect
+ change the conversion to Steel

experiment/Experiment.Steel.Effect.fst
@@ -28,32 +28,54 @@ irreducible let __mrepr_implicit__ : unit = ()
 unfold
 type prog_tree = M.prog_tree u#a u#8
 
-type repr' (a : Type) (ek : SH.effect_kind) (t : M.prog_tree u#a u#p a) : Type
+type repr_eq (a : Type) (ek : SH.effect_kind) (t : M.prog_tree u#a u#p a) : Type
   = r : M.repr u#a u#p ek a { r.repr_tree == t }
 
-type repr (a : Type) (ek : SH.effect_kind) (t : prog_tree u#a a) : Type
-  = r : M.repr u#a u#8 ek a { r.repr_tree == t }
+type repr' = repr_eq u#a u#8
 
+/// We want to avoid a retypechecking of the [M.prog_tree] which may fail because of
+/// the monotonicity refinement on [pure_wp].
+/// For this reason, we convert our representation to Steel directly in the effect using a
+/// [repr_cv] field, which contains the conversion if the [cvi] index is set to some
+/// specification.
+
+noeq
+type conv_index (a : Type u#a) = {
+  cvi_pre   : SE.pre_t;
+  cvi_post  : SE.post_t a;
+  cvi_req   : SE.req_t cvi_pre;
+  cvi_ens   : SE.ens_t cvi_pre a cvi_post;
+  cvi_flags : list flag;
+}
+
+noeq
+type indexed_option (a : Type) (f : a -> Type) : option a -> Type =
+  | ISome : (x : a) -> (v : f x) -> indexed_option a f (Some x)
+  | INone : indexed_option a f None
+
+noeq
+type repr (a : Type) (ek : SH.effect_kind) (t : prog_tree a) (cvi : option (conv_index a)) =
+  {
+    repr_M  : repr' a ek t;
+    repr_cv : indexed_option
+                (conv_index a) (fun c -> SH.steel a c.cvi_pre c.cvi_post c.cvi_req c.cvi_ens ek)
+                cvi
+  }
+
+let mk_repr (#a : Type) (#ek : SH.effect_kind) (#t : prog_tree a) (repr_M : repr' a ek t)
+  : repr a ek t None
+  = {
+    repr_M;
+    repr_cv = INone
+  }
 
 (***** return *)
 
 let return_ghostI
-      (a : Type) (x : a) (#opened: Mem.inames)
-  : repr u#a a (SH.KGhostI opened) (M.Tret a x (fun _ -> []))
-  = C.return_ghostI_hint #a x (fun _ -> [])
-
-let return_ghost
-      (a : Type) (x : a) (#opened: Mem.inames)
-  : repr u#a a (SH.KGhost opened) (M.Tret a x (fun _ -> []))
-  = C.return_ghost #a x
-
-// FIXME
-//   if we replace SH.KGhostI by SH.KGhost, [test3'] fails because of some bind
-//   maybe we can infer when one should use return_ghostI/return_ghost
-let return_
       (a : Type) (x : a) (#[@@@ __mrepr_implicit__] opened: Mem.inames)
-  : repr u#a a (SH.KGhostI opened) (M.Tret a x (fun _ -> []))
-  = return_ghostI a x #opened
+  : repr u#a a (SH.KGhostI opened) (M.Tret a x (fun _ -> [])) None
+  = mk_repr (C.return_ghostI_hint #a x (fun _ -> []))
+
 
 (***** bind *)
 
@@ -65,21 +87,27 @@ type combine_bind_t
        (f : prog_tree a) (g : a -> prog_tree b)
 = {
   cb_bind_repr : prog_tree b;
-  cb_bind_impl : (rf : repr a ek0 f) -> (rg : ((x : a) -> repr b ek1 (g x))) ->
-                 repr b ek cb_bind_repr
+  cb_bind_impl : (rf : repr' a ek0 f) -> (rg : ((x : a) -> repr' b ek1 (g x))) ->
+                 repr' b ek cb_bind_repr
 }
 
 type combinable_bind_repr (a0 a1 : Type u#a) (ek0 ek1 ek2 : SH.effect_kind)
   = (f : M.repr u#a u#8 ek0 a0) -> (g : ((x : a0) -> M.repr u#a u#8 ek1 a1)) ->
-    repr a1 ek2 (M.Tbind a0 a1 f.repr_tree (fun x -> (g x).repr_tree))
+    repr_eq a1 ek2 (M.Tbind a0 a1 f.repr_tree (fun x -> (g x).repr_tree))
+
+let repr_tree_eq #a #ek #t (r : repr_eq a ek t) : squash (r.repr_tree == t)
+  = ()
 
 noeq inline_for_extraction
 type combinable_bind_t (a0 a1 : Type u#a) (ek0 ek1 ek2 : SH.effect_kind) = {
   cba_bind_ek0'  : SH.effect_kind;
   cba_bind_ek1'  : SH.effect_kind;
-  cba_bind_repr  : combinable_bind_repr a0 a1 cba_bind_ek0' cba_bind_ek1' ek2;
+  // Sometime ek2 has already been resolved (for instance in test9', don't know why)
+  cba_bind_ek2'  : SH.effect_kind;
+  cba_bind_repr  : combinable_bind_repr a0 a1 cba_bind_ek0' cba_bind_ek1' cba_bind_ek2';
   cba_bind_lift0 : C.steel_liftable a0 ek0 cba_bind_ek0';
   cba_bind_lift1 : C.steel_liftable a1 ek1 cba_bind_ek1';
+  cba_bind_lift2 : C.steel_liftable a1 cba_bind_ek2' ek2;
 }
 
 [@@ __repr_M__]
@@ -90,15 +118,27 @@ let combine_bind
       (cba : combinable_bind_t a b ek0 ek1 ek2)
       (f : prog_tree a) (g : a -> prog_tree b)
   : combine_bind_t a b ek0 ek1 ek2 f g
-  = {
-    cb_bind_repr = M.Tbind a b f (fun x -> g x); // We need the functional extensionality so we eta-expend g
+  =
+    let t = M.Tbind a b f (fun x -> g x) in // We need the functional extensionality so we eta-expend g
+  {
+    cb_bind_repr = t;
     cb_bind_impl = (fun rf rg ->
-                      let rf' = C.repr_lift cba.cba_bind_lift0 rf             in
-                      let rg' (x : a) = C.repr_lift cba.cba_bind_lift1 (rg x) in
+                      let rf' = C.repr_lift cba.cba_bind_lift0 rf                        in
+                      let rg' (x : a) = C.repr_lift cba.cba_bind_lift1 (rg x)            in
+                      let r = C.repr_lift cba.cba_bind_lift2 (cba.cba_bind_repr rf' rg') in
                       U.funext_eta (fun x -> g x) (fun x -> (rg' x).repr_tree)
                         (U.by_refl ()) (U.by_refl ())
                         (fun x -> ());
-                      cba.cba_bind_repr rf' rg');
+                      calc (==) {
+                        r.repr_tree;
+                      == { }
+                        (cba.cba_bind_repr rf' rg').repr_tree;
+                      == { _ by T.(apply (`repr_tree_eq)) }
+                        M.Tbind a b rf'.repr_tree (fun x -> (rg' x).repr_tree);
+                      == { }
+                        t;
+                      };
+                      r);
   }
 
 /// Since we want to represent the program as a tree, we need [u#a == u#b]. However when defining an effect,
@@ -113,40 +153,87 @@ let bind_
       (#f : prog_tree a) (#g : a -> prog_tree b)
       (#[@@@ __mrepr_implicit__] cb
         : (f : prog_tree a) -> (g : (a -> prog_tree b)) -> combine_bind_t a b ek0 ek1 ek f g)
-      (rf : repr u#a a ek0 f) (rg : (x : a) -> repr u#b b ek1 (g x))
-  : repr u#b b ek (cb f g).cb_bind_repr
-  = (cb f g).cb_bind_impl rf rg
+      (rf : repr u#a a ek0 f None) (rg : (x : a) -> repr u#b b ek1 (g x) None)
+  : repr u#b b ek (cb f g).cb_bind_repr None
+  = mk_repr ((cb f g).cb_bind_impl rf.repr_M (fun x -> (rg x).repr_M))
 
 
 (***** subcomp *)
 
+noeq
 type combine_subcomp_t
       (a : Type u#a) (ek0 ek1 : SH.effect_kind) (f : prog_tree a) (g : prog_tree a)
-  = repr a ek0 f -> repr a ek1 g
+      (cvi : option (conv_index a))
+  = {
+    cba_subc : repr a ek0 f None -> repr a ek1 g cvi;
+  }
 
-// TODO?: allow lifting effect_kind
 let combine_subcomp_refl
       (a : Type u#a) (ek : SH.effect_kind) (f : prog_tree a)
-  : combine_subcomp_t a ek ek f f
-  = fun rf -> rf
+  : combine_subcomp_t a ek ek f f None
+  = Mkcombine_subcomp_t (fun rf -> rf)
+
+noeq
+type mrepr_to_steel_t
+       (flags : list flag)
+       (a : Type) (ek : SH.effect_kind)
+       (pre : SE.pre_t) (post : SE.post_t a) (req : SE.req_t pre) (ens : SE.ens_t pre a post)
+       (t : prog_tree a)
+  = | MReprToSteel of (repr' a ek t -> SH.steel a pre post req ens ek)
+
+private
+type dummy_spec (a : Type u#a) (sp : M.spec_r a) : Type u#b =
+
+private
+let dummy_prog_tree (a : Type u#a) : prog_tree a
+  = M.Tspec a (dummy_spec a)
+
+private
+let dummy_repr (a : Type u#a) (ek : SH.effect_kind) : repr' a ek (dummy_prog_tree a)
+  = {
+    repr_tree  = dummy_prog_tree a;
+    repr_steel = (fun pre post c -> false_elim ())
+  }
+
+/// This subcomp is used at top-level, to convert our representation to Steel. To avoid the retypechecking of
+/// [t], we replace it with [dummy_prog_tree].
+let combine_subcomp_convert
+      (a : Type u#a) (ek0 ek1 : SH.effect_kind) (t : prog_tree a)
+      (pre : SE.pre_t) (post : SE.post_t a) (req : SE.req_t pre) (ens : SE.ens_t pre a post) (flags : list flag)
+      (lt : C.steel_liftable a ek0 ek1)
+      (cv : mrepr_to_steel_t flags a ek1 pre post req ens t)
+  : combine_subcomp_t a ek0 ek1 t (dummy_prog_tree a) (Some (Mkconv_index pre post req ens flags))
+  = Mkcombine_subcomp_t (fun r ->
+      let r' = C.repr_lift lt r.repr_M in
+      let MReprToSteel cv = cv in
+      {
+        repr_M = dummy_repr a ek1;
+        repr_cv = ISome _ (cv r')
+      })
 
 let subcomp
       (a : Type u#a)
       (#ek0 : SH.effect_kind) (#ek1 : SH.effect_kind)
       (#f : prog_tree a) (#g : prog_tree a)
-      (#[@@@ __mrepr_implicit__] cb : combine_subcomp_t a ek0 ek1 f g)
-      (rf : repr a ek0 f)
-  : repr a ek1 g
-  = cb rf
+      (cvi : option (conv_index a))
+      (#[@@@ __mrepr_implicit__] cb : combine_subcomp_t a ek0 ek1 f g cvi)
+      (rf : repr a ek0 f None)
+  : repr a ek1 g cvi
+  = cb.cba_subc rf
 
 
 (***** if then else *)
 
+// We match the restriction of SteelAtomic, but we do not need it
+type cba_ite_effect_kind_t =
+  ek : SH.effect_kind { ~ (SH.KAtomic? ek) }
+
 noeq
 type combinable_ite_t (a : Type) (ek0 ek1 ek2 : SH.effect_kind) = {
-  cba_ite_restr : squash (~ (SH.KAtomic? ek2)); // We match the restriction of SteelAtomic, but we do not need it
-  cba_ite_lift0 : C.steel_liftable a ek0 ek2;
-  cba_ite_lift1 : C.steel_liftable a ek1 ek2;
+  cba_ite_ek2'  : cba_ite_effect_kind_t;
+  cba_ite_lift0 : C.steel_liftable a ek0 cba_ite_ek2';
+  cba_ite_lift1 : C.steel_liftable a ek1 cba_ite_ek2';
+  cba_ite_lift2 : C.steel_liftable a cba_ite_ek2' ek2;
 }
 
 let if_then_else
@@ -154,10 +241,10 @@ let if_then_else
       (#ek0 #ek1 #ek2 : SH.effect_kind)
       (#thn : prog_tree a) (#els : prog_tree a)
       (#[@@@ __mrepr_implicit__] cb : combinable_ite_t a ek0 ek1 ek2)
-      (rthn : repr a ek0 thn) (rels : repr a ek1 els)
+      (rthn : repr a ek0 thn None) (rels : repr a ek1 els None)
       (guard : bool)
   : Type
-  = repr a ek2 (M.Tif a guard thn els)
+  = repr a ek2 (M.Tif a guard thn els) None
 
 
 inline_for_extraction noextract
@@ -182,30 +269,30 @@ let ite_steel_els
 
 
 let ite_combine_thn
-      (a : Type) (ek0 ek1 : SH.effect_kind) (guard : bool) (thn els : prog_tree a)
+      (a : Type) (ek0 ek1 ek2 : SH.effect_kind) (guard : bool) (thn els : prog_tree a)
       (_ : squash guard)
-      (l : C.steel_liftable a ek0 ek1)
-  : combine_subcomp_t a ek0 ek1 thn (M.Tif a guard thn els)
-  = fun rthn -> {
+      (l0 : C.steel_liftable a ek0 ek1) (l1 : C.steel_liftable a ek1 ek2)
+  : combine_subcomp_t a ek0 ek2 thn (M.Tif a guard thn els) None
+  = Mkcombine_subcomp_t (fun rthn -> mk_repr ({
     repr_tree  = M.Tif a guard thn els;
     repr_steel = (fun pre0 post0 c ->
                     let M.TCif pre post cthn cels = c in
-                    ite_steel_thn a ek1 guard thn els pre post cthn cels
-                         ((C.repr_lift l rthn).repr_steel _ _  cthn) ())
-  }
+                    ite_steel_thn a ek2 guard thn els pre post cthn cels
+                         ((C.repr_lift l1 (C.repr_lift l0 rthn.repr_M)).repr_steel _ _  cthn) ())
+  }))
 
 let ite_combine_els
-      (a : Type) (ek0 ek1 : SH.effect_kind) (guard : bool) (thn els : prog_tree a)
+      (a : Type) (ek0 ek1 ek2 : SH.effect_kind) (guard : bool) (thn els : prog_tree a)
       (_ : squash (~guard))
-      (l : C.steel_liftable a ek0 ek1)
-  : combine_subcomp_t a ek0 ek1 els (M.Tif a guard thn els)
-  = fun rels -> {
+      (l0 : C.steel_liftable a ek0 ek1) (l1 : C.steel_liftable a ek1 ek2)
+  : combine_subcomp_t a ek0 ek2 els (M.Tif a guard thn els) None
+  = Mkcombine_subcomp_t (fun rels -> mk_repr ({
     repr_tree  = M.Tif a guard thn els;
     repr_steel = (fun pre0 post0 c ->
                     let M.TCif pre post cthn cels = c in
-                    ite_steel_els a ek1 guard thn els pre post cthn cels
-                          ((C.repr_lift l rels).repr_steel _ _ cels) ())
-  }
+                    ite_steel_els a ek2 guard thn els pre post cthn cels
+                          ((C.repr_lift l1 (C.repr_lift l0 rels.repr_M)).repr_steel _ _ cels) ())
+  }))
 
 
 private irreducible
@@ -224,29 +311,26 @@ let ite_soundness_tac () : T.Tac unit
     first [
       (fun () -> apply (`Mkcombinable_ite_t?.cba_ite_lift0); exact_hyp ());
       (fun () -> apply (`Mkcombinable_ite_t?.cba_ite_lift1); exact_hyp ())
-    ]
+    ];
+    apply (`Mkcombinable_ite_t?.cba_ite_lift2)
   )
 
 
-[@@ ite_soundness_by __ite_soundness__]
-total reflectable effect {
-  MRepr (a : Type) (ek : SH.effect_kind) (r : prog_tree a)
+[@@ ite_soundness_by __ite_soundness__; allow_informative_binders]
+total reflectable reifiable effect {
+  MRepr (a : Type) (ek : SH.effect_kind) (t : prog_tree a) (cvi : option (conv_index a))
   with {
     repr;
-    return = return_;
-    bind = bind_;
+    return = return_ghostI;
+    bind   = bind_;
     subcomp;
-    if_then_else
+    if_then_else;
   }
 }
 
 let return (#a : Type u#a) (#opened : Mem.inames) (x : a)
-  : MRepr a (SH.KGhostI opened) (M.Tret a x (fun _ -> []))
+  : MRepr a (SH.KGhostI opened) (M.Tret a x (fun _ -> [])) None
   = MRepr?.reflect (return_ghostI a x #opened)
-
-let return_g (#a : Type u#a) (#opened : Mem.inames) (x : a)
-  : MRepr a (SH.KGhost opened) (M.Tret a x (fun _ -> []))
-  = MRepr?.reflect (return_ghost a x #opened)
 
 
 (***** bind (PURE, MRepr) |> MRepr *)
@@ -259,8 +343,8 @@ type combine_bind_pure_t
        (wp : pure_wp a) (g : a -> M.prog_tree u#a u#p b)
 = {
   cb_bindP_repr : M.prog_tree u#a u#p b;
-  cb_bindP_impl : (rf : unit -> PURE a wp) -> (rg : ((x : a) -> repr' b ek (g x))) ->
-                  repr' u#a u#p b ek cb_bindP_repr
+  cb_bindP_impl : (rf : unit -> PURE a wp) -> (rg : ((x : a) -> repr_eq b ek (g x))) ->
+                  repr_eq u#a u#p b ek cb_bindP_repr
 }
 
 /// This should be applied with [u#r <= u#8] so [u#(max r 8) = u#8]
@@ -300,20 +384,114 @@ let bind_pure_mrepr
       (#[@@@ __mrepr_implicit__] cb
         : (wp : pure_wp a) -> (g : (a -> prog_tree b)) -> combine_bind_pure_t u#r u#a u#8 a b ek wp g)
       (rf : eqtype_as_type unit -> PURE a wp)
-      (rg : (x : a) -> repr b ek (g x))
-  : repr b ek (cb wp g).cb_bindP_repr
-  = (cb wp g).cb_bindP_impl rf rg
+      (rg : (x : a) -> repr b ek (g x) None)
+  : repr b ek (cb wp g).cb_bindP_repr None
+  = mk_repr ((cb wp g).cb_bindP_impl rf (fun x -> (rg x).repr_M))
 
 #push-options "--warn_error -330"
 polymonadic_bind (PURE, MRepr) |> MRepr = bind_pure_mrepr
 #pop-options
 
 
-(***** lifting Steel ~> MRepr *)
+(**** MReprGhost effect *)
+
+/// In order to be able to use ghost operation in SteelGhost operations, we declare a MReprGhost effect, with the
+/// same representation as MRepr, but with the effect_kind fixed to [KGhost] and declared as erasable.
+/// We do not use new_effect in order to change the effect_kind of the return combinator.
+// ALT: fix the combinator (bind, if then else) in the effect instead of relying on tactics to always infer
+//      the ghost combinator
+
+type repr_ghost (a : Type u#a) (opened : Mem.inames) (t : prog_tree a) (cvi : option (conv_index a)) =
+  repr a (SH.KGhost opened) t cvi
+
+let return_ghost
+      (a : Type) (x : a) (#opened: Mem.inames)
+  : repr_ghost u#a a opened (M.Tret a x (fun _ -> [])) None
+  = mk_repr (C.return_ghost #a x)
+
+let bind_ghost
+      (a : Type u#a) (b : Type u#b)
+      (#o : Mem.inames)
+      (#f : prog_tree a) (#g : a -> prog_tree b)
+      (#[@@@ __mrepr_implicit__] cb
+        : (f : prog_tree a) -> (g : (a -> prog_tree b)) ->
+          combine_bind_t a b (SH.KGhost o) (SH.KGhost o) (SH.KGhost o) f g)
+      (rf : repr_ghost u#a a o f None) (rg : (x : a) -> repr_ghost u#b b o (g x) None)
+  : repr_ghost u#b b o (cb f g).cb_bind_repr None
+  = mk_repr ((cb f g).cb_bind_impl rf.repr_M (fun x -> (rg x).repr_M))
+
+let subcomp_ghost
+      (a : Type u#a)
+      (#o : Mem.inames)
+      (#f : prog_tree a) (#g : prog_tree a)
+      (cvi : option (conv_index a))
+      (#[@@@ __mrepr_implicit__] cb : combine_subcomp_t a (SH.KGhost o) (SH.KGhost o) f g cvi)
+      (rf : repr_ghost a o f None)
+  : repr_ghost a o g cvi
+  = cb.cba_subc rf
+
+let if_then_else_ghost
+      (a : Type)
+      (#o : Mem.inames)
+      (#thn : prog_tree a) (#els : prog_tree a)
+      (#[@@@ __mrepr_implicit__] cb : combinable_ite_t a (SH.KGhost o) (SH.KGhost o) (SH.KGhost o))
+      (rthn : repr_ghost a o thn None) (rels : repr_ghost a o els None)
+      (guard : bool)
+  : Type
+  = repr_ghost a o (M.Tif a guard thn els) None
+
+
+[@@ erasable; ite_soundness_by __ite_soundness__; allow_informative_binders]
+total reflectable reifiable effect {
+  MReprGhost (a : Type) (opened : Mem.inames) (t : prog_tree a) (cvi : option (conv_index a))
+  with {
+    repr         = repr_ghost;
+    return       = return_ghost;
+    bind         = bind_ghost;
+    subcomp      = subcomp_ghost;
+    if_then_else = if_then_else_ghost;
+  }
+}
+
+let return_g (#a : Type u#a) (#opened : Mem.inames) (x : a)
+  : MReprGhost a opened (M.Tret a x (fun _ -> [])) None
+  = MReprGhost?.reflect (return_ghost a x #opened)
+
+let bind_pure_mrepr_ghost
+      (a : Type u#r) (b : Type u#a)
+      (#o : Mem.inames)
+      (#wp : pure_wp a)
+      (#g : a -> prog_tree b)
+      (#[@@@ __mrepr_implicit__] cb
+        : (wp : pure_wp a) -> (g : (a -> prog_tree b)) -> combine_bind_pure_t u#r u#a u#8 a b (SH.KGhost o) wp g)
+      (rf : eqtype_as_type unit -> PURE a wp)
+      (rg : (x : a) -> repr_ghost b o (g x) None)
+  : repr_ghost b o (cb wp g).cb_bindP_repr None
+  = mk_repr ((cb wp g).cb_bindP_impl rf (fun x -> (rg x).repr_M))
+
+#push-options "--warn_error -330"
+polymonadic_bind (PURE, MReprGhost) |> MReprGhost = bind_pure_mrepr_ghost
+#pop-options
+
+/// The [steel_liftable] condition is equivalent to [C.erasable_t a].
+/// If [a] is not erasable F* should raise an error when using this lift but since [repr_ghost] is a
+/// SteelGhost and [repr _ (SH.KGhostI) _] is a SteelAGcommon, we still need to do our own lift.
+let lift_mrepr_ghost_mrepr
+      (a : Type) (opened: Mem.inames)
+      (#t : prog_tree a)
+      (#[@@@ __mrepr_implicit__] lt : C.steel_liftable a (SH.KGhost opened) (SH.KGhostI opened))
+      (r : repr_ghost a opened t None)
+  : repr a (SH.KGhostI opened) t None
+  = mk_repr (C.repr_lift lt r.repr_M)
+
+sub_effect MReprGhost ~> MRepr = lift_mrepr_ghost_mrepr
+
+
+(**** lifting Steel ~> MRepr *)
 
 /// The sub_effect is not working (order of resolution of the implicits, use of Steel's combinators instead of
 /// MRepr's combinators, Steel computation unexpectedly lifted where MRepr does not appear).
-/// One has use an explicit cast ([call]) instead.
+/// One has to use an explicit cast ([call]) instead.
 
 (*
 let lift_steel_mrepr
@@ -332,111 +510,16 @@ let call (#b : Type u#b)
       (#a : b -> Type) (#pre : b -> SE.pre_t) (#post : (x : b) -> SE.post_t (a x))
       (#req : (x : b) -> SE.req_t (pre x)) (#ens : (x : b) -> SE.ens_t (pre x) (a x) (post x))
       ($f : (x : b) -> SE.Steel (a x) (pre x) (post x) (req x) (ens x)) (x : b)
-  : MRepr (a x) SH.KSteel (M.Tspec (a x) (M.spec_r_steel u#a u#8 (pre x) (post x) (req x) (ens x)))
-  = MRepr?.reflect (C.repr_of_steel #(a x) (pre x) (post x) (req x) (ens x) (fun () -> f x))
+  : MRepr (a x) SH.KSteel (M.Tspec (a x) (M.spec_r_steel u#a u#8 (pre x) (post x) (req x) (ens x))) None
+  = MRepr?.reflect (mk_repr (C.repr_of_steel #(a x) (pre x) (post x) (req x) (ens x) (fun () -> f x)))
 
 unfold
 let call_g (#b : Type u#b)
       (#a : b -> Type) (#opened : b -> Mem.inames) (#pre : b -> SE.pre_t) (#post : (x : b) -> SE.post_t (a x))
       (#req : (x : b) -> SE.req_t (pre x)) (#ens : (x : b) -> SE.ens_t (pre x) (a x) (post x))
       ($f : (x : b) -> SA.SteelGhost (a x) (opened x) (pre x) (post x) (req x) (ens x)) (x : b)
-  : MRepr (a x) (SH.KGhost (opened x)) (M.Tspec (a x) (M.spec_r_steel u#a u#8 (pre x) (post x) (req x) (ens x)))
-  = MRepr?.reflect (C.repr_of_steel_ghost #(a x) (pre x) (post x) (req x) (ens x) (fun () -> f x))
-
-
-(*** Conversion to Steel *)
-
-/// [ConvEffect] is a dummy effect whose only purpose is to avoid the retypechecking of [prog_tree] that would
-/// happen if it appeared outside effect combinators.
-
-type cv_repr (a : Type u#a) (ek : SH.effect_kind) (pre : SE.pre_t) (post : SE.post_t a)
-             (req : SE.req_t pre) (ens : SE.ens_t pre a post)
-             (flags : list flag)
-  : Type
-  = SH.steel a pre post req ens ek
-
-/// [ConvEffect] is only used to convert a [MRepr] into a [SH.unit_steel]. Its combinators (return, bind,
-/// lifting of pure) should never be used.
-
-irreducible let __cv_unused__ : unit = ()
-
-[@@ resolve_implicits; __cv_unused__]
-let cv_unused_tac () : T.Tac unit
-  = T.fail "cv_unused"
-
-[@@ erasable]
-noeq type cv_unused =
-
-let elim_cv_unused (#a : Type) (u : cv_unused) : a
-  = match u with
-
-unfold let dummy_cv (a : Type u#a) = cv_repr a SH.KSteel SE.emp (fun _ -> SE.emp) (fun _ -> True) (fun _ _ _ -> True) []
-
-let cv_return
-      (a : Type u#a) (x : a) (#[@@@ __cv_unused__] u : cv_unused)
-  : dummy_cv a
-  = elim_cv_unused u
-
-let cv_bind
-      (a : Type u#a) (b : Type u#b)
-      (#ek0 #ek1 : SH.effect_kind)
-      (#pre_f : SE.pre_t) (#post_f : SE.post_t a)
-      (#req_f : SE.req_t pre_f) (#ens_f : SE.ens_t pre_f a post_f)
-      (#fsf : list flag)
-      (#pre_g : a -> SE.pre_t) (#post_g : a -> SE.post_t b)
-      (#req_g : (x : a) -> SE.req_t (pre_g x)) (#ens_g : (x : a) -> SE.ens_t (pre_g x) b (post_g x))
-      (#fsg : (x : a) -> list flag)
-      (#[@@@ __cv_unused__] u : cv_unused)
-      (f : cv_repr a ek0 pre_f post_f req_f ens_f fsf)
-      (g : (x : a) -> cv_repr b ek1 (pre_g x) (post_g x) (req_g x) (ens_g x) (fsg x))
-  : dummy_cv b
-  = elim_cv_unused u
-
-/// We need the reification for extracting the Steel representation and [lift_mrepr_cv] has [t : prog_tree a]
-/// as an informative binder. (ALT? make [prog_tree] erasable)
-[@@ allow_informative_binders]
-total reifiable effect {
-  ConvEffect
-    (a : Type) (ek : SH.effect_kind) (pre : SE.pre_t) (post : SE.post_t a)
-    (req : SE.req_t pre) (ens : SE.ens_t pre a post)
-    (flags : list flag)
-  with {
-    repr   = cv_repr;
-    return = cv_return;
-    bind   = cv_bind;
-  }
-}
-
-
-let lift_pure_cv
-      (a : Type) (wp : pure_wp a)
-      (#[@@@ __cv_unused__] u : cv_unused)
-      (f : (eqtype_as_type unit) -> PURE a wp)
-  : Tot (dummy_cv a)
-  = elim_cv_unused u
-
-sub_effect PURE ~> ConvEffect = lift_pure_cv
-
-
-noeq
-type mrepr_to_steel_t
-       (flags : list flag)
-       (a : Type) (ek : SH.effect_kind)
-       (pre : SE.pre_t) (post : SE.post_t a) (req : SE.req_t pre) (ens : SE.ens_t pre a post)
-       (t : prog_tree a)
-  = | MReprToSteel of (repr a ek t -> SH.steel a pre post req ens ek)
-
-let lift_mrepr_cv
-      (a : Type) (ek0 ek1 : SH.effect_kind) (t : prog_tree a)
-      (pre : SE.pre_t) (post : SE.post_t a) (req : SE.req_t pre) (ens : SE.ens_t pre a post) (flags : list flag)
-      ([@@@ __mrepr_implicit__] lt : C.steel_liftable a ek0 ek1)
-      ([@@@ __mrepr_implicit__] cv : mrepr_to_steel_t flags a ek1 pre post req ens t)
-      (r : repr a ek0 t)
-  : cv_repr a ek1 pre post req ens flags
-  = let MReprToSteel cv = cv in
-    cv (C.repr_lift lt r)
-
-sub_effect MRepr ~> ConvEffect = lift_mrepr_cv
+  : MReprGhost (a x) (opened x) (M.Tspec (a x) (M.spec_r_steel u#a u#8 (pre x) (post x) (req x) (ens x))) None
+  = MReprGhost?.reflect (mk_repr (C.repr_of_steel_ghost #(a x) (pre x) (post x) (req x) (ens x) (fun () -> f x)))
 
 
 (*** Implicits resolution *)
@@ -450,15 +533,20 @@ open Learn.Tactics.Util
 
 // TODO: better errors
 
+(***** stage 1 *)
+
 private noeq
 type filter_goals_r = {
   // combinable_bind_t, combinable_ite_t
   fgoals_comb : list goal;
   // steel_liftable
   fgoals_lift : list goal;
-  // mrepr_to_steel_t
-  fgoals_tstl : list goal;
+  // combine_subcomp_t
+  fgoals_subc : list goal;
 }
+
+let remove_already_solved () : Tac unit =
+  iterAll (fun () -> if not (Tv_Uvar? (cur_witness ())) then dismiss ())
 
 let rec mrepr_implicits_init (r : filter_goals_r) : Tac filter_goals_r
   =
@@ -476,22 +564,20 @@ let rec mrepr_implicits_init (r : filter_goals_r) : Tac filter_goals_r
           // different universes. Or a polymonadic bind with an universe greater than [u#8].
           if hd = (`%combine_bind_t)
           then begin
-            apply (`combine_bind);
-            // combinable_bind_t
-            let g = _cur_goal () in
-            dismiss ();
-            {r with fgoals_comb = g :: r.fgoals_comb}
-          end else if hd = (`%combine_subcomp_t)
-          then (apply (`combine_subcomp_refl); r)
-          else if hd = (`%combine_bind_pure_t)
+              apply (`combine_bind);
+              // combinable_bind_t
+              let g = _cur_goal () in
+              dismiss ();
+              {r with fgoals_comb = g :: r.fgoals_comb}
+          end else if hd = (`%combine_bind_pure_t)
           then (apply (`combine_bind_pure); r)
 
           else if hd = (`%combinable_ite_t)
           then (dismiss (); {r with fgoals_comb = g :: r.fgoals_comb})
           else if hd = (`%C.steel_liftable)
           then (dismiss (); {r with fgoals_lift = g :: r.fgoals_lift})
-          else if hd = (`%mrepr_to_steel_t)
-          then (dismiss (); {r with fgoals_tstl = g :: r.fgoals_tstl})
+          else if hd = (`%combine_subcomp_t)
+          then (dismiss (); {r with fgoals_subc = g :: r.fgoals_subc})
           else if hd = (`%Mem.inames)
           then (dismiss (); r) // should be inferred as side effects of other goals
           else fail "unexpected shape"
@@ -499,8 +585,10 @@ let rec mrepr_implicits_init (r : filter_goals_r) : Tac filter_goals_r
       in
       mrepr_implicits_init r
 
+(***** stage 2 *)
 
-/// Solves a goal [C.steel_liftable a ek0 ek1] where the heads of [ek0] and [ek1] are known.
+/// Solves a goal [C.steel_liftable a ek0 ek1].
+/// Since we start by trying to apply [C.Rt1n_refl], if [ek0] or [ek1] is an uvar, we will choose a trivial lift.
 let rec build_steel_liftable () : Tac unit
   =
     try apply (`C.Rt1n_refl)
@@ -588,17 +676,11 @@ let combinable_bind_op (ek0 ek1 : effect_kind_enum) : term
   | ESteel  -> (`combinable_bind_steel)
 
 
-private
-let __build_combinable_ite_t
-      (ek2 : SH.effect_kind{~ (SH.KAtomic? ek2)}) (a : Type) (ek0 ek1 : SH.effect_kind)
-      (lt0 : C.steel_liftable a ek0 ek2) (lt1 : C.steel_liftable a ek1 ek2)
-  = Mkcombinable_ite_t #a #ek0 #ek1 #ek2 () lt0 lt1
+let combinable_ite_ghost  o : cba_ite_effect_kind_t =  SH.KGhost  o
+let combinable_ite_ghostI o : cba_ite_effect_kind_t = (SH.KGhostI o)
+let combinable_ite_steel    : cba_ite_effect_kind_t =  SH.KSteel
 
-let combinable_ite_ghost  o = __build_combinable_ite_t (SH.KGhost  o)
-let combinable_ite_ghostI o = __build_combinable_ite_t (SH.KGhostI o)
-let combinable_ite_steel    = __build_combinable_ite_t  SH.KSteel
-
-let combinable_ite_op (ek0 ek1 : effect_kind_enum) : term
+let combinable_ite_kind (ek0 ek1 : effect_kind_enum) : term
   = match if ek0 `ek_le` ek1 then ek1 else ek0 with
   | EGhost  -> (`combinable_ite_ghost)
   | EGhostI -> (`combinable_ite_ghostI)
@@ -622,10 +704,12 @@ let build_combinable () : Tac bool
              let op = combinable_bind_op ek0 ek1 in
              apply (`Mkcombinable_bind_t);
              // cba_bind_repr
-             apply op;
+             seq (fun () -> apply op) dismiss;
              // cba_bind_lift0
              build_steel_liftable ();
              // cba_bind_lift1
+             build_steel_liftable ();
+             // cba_bind_lift2
              build_steel_liftable ();
              true
       | _ -> false
@@ -636,11 +720,15 @@ let build_combinable () : Tac bool
       let ek1 = collect_effect_kind (L.index args 2)._1 in
       match ek0, ek1 with
       | Some ek0, Some ek1 ->
-             let op = combinable_ite_op ek0 ek1 in
-             apply op;
+             let ek = combinable_ite_kind ek0 ek1 in
+             apply_raw (`Mkcombinable_ite_t);
+             // cba_ite_ek2'
+             seq (fun () -> apply ek) dismiss;
              // cba_ite_lift0
              build_steel_liftable ();
              // cba_ite_lift1
+             build_steel_liftable ();
+             // cba_ite_lift2
              build_steel_liftable ();
              true
       | _ -> false
@@ -668,6 +756,8 @@ let rec solve_combinables () : Tac unit
     if not b then fail "solve_combinables: could not progress";
     set_goals gs;
     solve_combinables ()
+
+(***** stage 3 *)
 
 private
 let __build_mrepr_to_steel_norew
@@ -720,7 +810,7 @@ let __build_mrepr_to_steel_wrew
 /// normalizing the WP twice.
 let build_mrepr_to_steel_wrew (fr : flags_record) (flags : list flag) : Tac unit
   =
-    let fr    = make_flags_record flags in
+    let fr = make_flags_record flags in
     apply_raw (`__build_mrepr_to_steel_wrew);
 
     // ek_restr
@@ -754,33 +844,42 @@ let build_mrepr_to_steel () : Tac unit
     then build_mrepr_to_steel_wrew  fr flags
     else build_mrepr_to_steel_norew fr
 
+/// Solves a goal [combine_subcomp_t a ek0 ek1 (ReprIM t) (ReprIS pre post req ens flag)]
+let solve_conversion_subcomp () : Tac unit
+  =
+    apply (`combine_subcomp_convert);
+    // lt
+    build_steel_liftable ();
+    // cv
+    build_mrepr_to_steel ()
+
+(***** entry *)
 
 [@@ resolve_implicits; __mrepr_implicit__]
 let mrepr_implicits_tac () : Tac unit
   = with_policy Force (fun () ->
 
     //let t = timer_start "implicits" true in
-
-    iterAll (fun () -> intros' (); try trefl () with _ -> ());
+    iterAll (fun () -> try trefl () with _ -> ());
+    iterAll intros';
     let fgoals = mrepr_implicits_init (Mkfilter_goals_r [] [] []) in
 
     // Solve the combinable_* goals
     set_goals fgoals.fgoals_comb;
     solve_combinables ();
 
-    // Solve the [steel_liftable] from the lifting to ConvEffect
+    // Solve the [steel_liftable] goals
     set_goals fgoals.fgoals_lift;
     iterAll build_steel_liftable;
 
     //timer_stop t;
 
-    
     // useful to debug `Tactic left uninstantiated unification variable` errors
     //dump_all true "implicits";
 
-    // Solve the [mrepr_to_steel_t] goal
-    set_goals fgoals.fgoals_tstl;
-    iterAll build_mrepr_to_steel
+    // Solve the [combine_subcomp_t] goals by building the conversion to Steel ([mrepr_to_steel_t])
+    set_goals fgoals.fgoals_subc;
+    iterAll solve_conversion_subcomp
   )
 
 
@@ -796,14 +895,20 @@ let usteel_ghost = SH.unit_steel_ghost
 let to_steel
       (#[apply (`[])] flags : list flag)
       (#a : Type) (#pre : SE.pre_t) (#post : SE.post_t a) (#req : SE.req_t pre) (#ens : SE.ens_t pre a post)
-      (r : unit -> ConvEffect a SH.KSteel pre post req ens flags)
+      (r : unit -> MRepr a SH.KSteel (dummy_prog_tree a) (Some (Mkconv_index pre post req ens flags)))
   : usteel a pre post req ens
-  = SH.steel_u (reify (r ()))
+  =
+    let r : repr a SH.KSteel (dummy_prog_tree a) (Some (Mkconv_index pre post req ens flags))
+      = reify (r ()) in
+    U.cast _ (SH.steel_u (ISome?.v r.repr_cv))
 
 let to_steel_g
       (#[apply (`[])] flags : list flag)
       (#a : Type) (#opened : Mem.inames)
       (#pre : SE.pre_t) (#post : SE.post_t a) (#req : SE.req_t pre) (#ens : SE.ens_t pre a post)
-      (r : unit -> ConvEffect a (SH.KGhost opened) pre post req ens flags)
+      (r : unit -> MReprGhost a opened (dummy_prog_tree a) (Some (Mkconv_index pre post req ens flags)))
   : usteel_ghost a opened pre post req ens
-  = SH.ghost_u (reify (r ()))
+  =
+    let r : repr a (SH.KGhost opened) (dummy_prog_tree a) (Some (Mkconv_index pre post req ens flags))
+      = reify (r ()) in
+    U.cast _ (SH.ghost_u (ISome?.v r.repr_cv))
